theories/TM/Compound/Shift.v
@@ -14,27 +14,37 @@ Local Arguments mult : simpl never.
 Section Shift.
 
   Variable sig : finType.
+  Variable (f : sig -> bool). (* halt if this symbol was read (and overwritten) *)
 
 
   Definition Shift_Step_Rel (s : sig) : pRel sig (sig + unit) 1 :=
     fun tin '(yout, tout) =>
       match current tin[@Fin0] with
-      | Some c => tout[@Fin0] = doAct tin[@Fin0] (Some s, R) /\ yout = inl c
+      | Some c =>
+        if f c
+        then tout[@Fin0] = doAct tin[@Fin0] (Some s, N) /\ yout = inr tt
+        else tout[@Fin0] = doAct tin[@Fin0] (Some s, R) /\ yout = inl c
       | None => tout[@Fin0] = tape_write tin[@Fin0] (Some s) /\ yout = inr tt
       end.
 
   Definition Shift_Step (s : sig) : pTM sig (sig + unit) 1 :=
     Switch (ReadChar)
            (fun c => match c with
-                  | Some c => Return (WriteMove s R) (inl c)
+                  | Some c =>
+                    if f c then Return (Write s) (inr tt)
+                    else Return (WriteMove s R) (inl c)
                   | None => Return (Write s) (inr tt)
                   end).
 
   Lemma Shift_Step_Sem (s : sig) : Shift_Step s ⊨c(3) Shift_Step_Rel s.
   Proof.
     eapply RealiseIn_monotone.
-    { unfold Shift_Step. TM_Correct. }
-    { Unshelve. 4,5: reflexivity. all: reflexivity. }
+    { unfold Shift_Step.
+      eapply Switch_RealiseIn with
+          (R2 := fun (c : option sig) => match c with Some c => if f c then _ else _ | None => _ end).
+      - TM_Correct.
+      - intros [ c | ]; [ destruct (f c) | ]; TM_Correct. }
+    { reflexivity. }
     {intros tin (yout, tout) H. TMSimp. TMCrush; TMSolve 1. }
   Qed.
 
@@ -46,7 +56,9 @@ Section Shift.
 
   Function Shift_fun (s : sig) (t : tape sig) {measure Shift_fun_measure t} :=
     match current t with
-    | Some c => Shift_fun c (doAct t (Some s, R))
+    | Some c =>
+      if f c then doAct t (Some s, N)
+      else Shift_fun c (doAct t (Some s, R))
     | None => tape_write t (Some s)
     end.
   Proof. intros. destruct t; cbn in *; inv teq. unfold Shift_fun_measure. simpl_tape. omega. Qed.
@@ -56,13 +68,16 @@ Section Shift.
 
   Lemma Shift_fun_move t s c :
     current t = Some c ->
+    f c = false ->
     Shift_fun c (tape_move_right' (left t) s (right t)) = Shift_fun s t.
   Proof.
-    intros HC. destruct t; cbn in *; inv HC. rename l into ls, l0 into rs.
-    revert ls s c. induction rs; intros; cbn in *.
-    - do 3 (rewrite Shift_fun_equation; cbn). reflexivity.
+    intros HC Hf. destruct t; cbn in *; inv HC. rename l into ls, l0 into rs.
+    revert ls s c Hf. induction rs; intros; cbn in *.
+    - do 3 (rewrite Shift_fun_equation; cbn). rewrite Hf. reflexivity.
     - rewrite Shift_fun_equation; cbn. symmetry. rewrite Shift_fun_equation; cbn. symmetry.
-      cbn. now rewrite IHrs.
+      cbn. rewrite !Hf; cbn.
+      destruct (f a) eqn:Ea; cbn in *; auto.
+      rewrite Shift_fun_equation; cbn; auto. now rewrite Ea.
   Qed.
 
   Lemma Shift_Realise (s : sig) : Shift s ⊨ Shift_Rel s.
@@ -71,26 +86,63 @@ Section Shift.
     { unfold Shift. TM_Correct. intros. eapply RealiseIn_Realise. apply Shift_Step_Sem. }
     {
       apply StateWhileInduction; intros; cbn in *.
-      - destruct (current tin[@Fin0]) eqn:E; destruct HLastStep as [HLastStep1 HLastStep2]; inv HLastStep2; TMSimp.
-        now rewrite Shift_fun_equation, E.
-      - destruct (current tin[@Fin0]) eqn:E; destruct HStar as [HStar1 HStar2]; inv HStar2; TMSimp.
-        now rewrite Shift_fun_move.
+      - destruct (current tin[@Fin0]) eqn:E.
+        + destruct (f e) eqn:Ee; TMSimp.
+          * now rewrite Shift_fun_equation, E, Ee.
+          * now rewrite Shift_fun_equation, E, Ee.
+        + now rewrite Shift_fun_equation, E.
+      - destruct (current tin[@Fin0]) eqn:E.
+        + destruct (f e) eqn:Ee; TMSimp; inv H0.
+          symmetry. now rewrite Shift_fun_equation, E, Ee.
+        + now rewrite Shift_fun_equation, E.
     }
   Qed.
 
 
   Lemma Shift_fun_correct_midtape s ls m rs r :
+    f m = false ->
+    f r = false ->
+    (forall x, In x rs -> f x = false) ->
     Shift_fun s (midtape ls m (rs ++ [r])) =
     midtape (rev rs ++ m :: s :: ls) r nil.
   Proof.
     revert s ls m. induction rs as [ | r' rs IH]; intros; cbn in *.
-    - do 3 (rewrite Shift_fun_equation; cbn). reflexivity.
-    - do 1 (rewrite Shift_fun_equation; cbn). rewrite <- !app_assoc. cbn. now rewrite IH.
+    - do 3 (rewrite Shift_fun_equation; cbn). rewrite H, H0. reflexivity.
+    - do 1 (rewrite Shift_fun_equation; cbn). rewrite <- !app_assoc. cbn. rewrite H. rewrite IH; eauto.
   Qed.
+
+  Lemma Shift_fun_correct_midtape_stop s ls m rs r h rs' :
+    f m = false ->
+    f r = false ->
+    f h = true ->
+    (forall x, In x rs -> f x = false) ->
+    Shift_fun s (midtape ls m (rs ++ r :: h :: rs')) =
+    midtape (rev rs ++ m :: s :: ls) r rs'.
+  Proof.
+    revert s ls m. induction rs as [ | r' rs IH]; intros; cbn in *.
+    - do 3 (rewrite Shift_fun_equation; cbn). rewrite H, H0, H1. reflexivity.
+    - do 1 (rewrite Shift_fun_equation; cbn). rewrite <- !app_assoc. cbn. rewrite H. rewrite IH; eauto.
+  Qed.
+
+  Fixpoint Shift_steps (rs : list sig) :=
+    match rs with
+    | nil => 4
+    | c :: rs => if f c then 4
+                else 4 + Shift_steps rs
+    end.
+
+  Lemma Shift_steps_local (rs : list sig) :
+    Shift_steps rs <= 4 + 4 * length rs.
+  Proof.
+    induction rs; cbn in *.
+    - omega.
+    - destruct (f a); omega.
+  Qed.
+
 
   Lemma Shift_TerminatesIn (s : sig) :
     projT1 (Shift s) ↓
-           (fun tin k => 4 + 4 * length (tape_local tin[@Fin0]) <= k).
+           (fun tin k => Shift_steps (tape_local tin[@Fin0]) <= k).
   Proof.
     eapply TerminatesIn_monotone.
     { unfold Shift. TM_Correct.
@@ -100,11 +152,16 @@ Section Shift.
     {
       revert s. apply StateWhileCoInduction; intros s; intros. exists 3. split. reflexivity.
       intros [ s' | [] ]; intros; cbn in *.
-      - destruct (current tin[@Fin0]) eqn:E; destruct H as [H1 H2]; inv H2; TMSimp. simpl_tape.
-        destruct tin[@Fin0] eqn:E'; cbn in *; inv E. rename l into ls, l0 into rs.
-        exists (4 + 4 * |rs|). split. reflexivity. omega.
-      - destruct (current tin[@Fin0]) eqn:E; destruct H as [H1 H2]; inv H2; TMSimp.
-        apply tape_local_nil in E. TMSimp. omega.
+      - destruct (current tin[@Fin0]) eqn:E.
+        + destruct (f e) eqn:Ee; destruct H as [H H']; inv H'.
+          destruct tin[@Fin0] eqn:E'; cbn in *; inv E. rename l into ls, l0 into rs.
+          TMSimp. simpl_tape. eexists. split. reflexivity. omega.
+        + destruct H. congruence.
+      - destruct (current tin[@Fin0]) eqn:E.
+        + destruct (f e) eqn:Ee; destruct H as [H H']; inv H'.
+          destruct tin[@Fin0] eqn:E'; cbn in *; inv E. rename l into ls, l0 into rs.
+          rewrite Ee in *. omega.
+        + apply tape_local_nil in E. TMSimp. omega.
     }
   Qed.
 
@@ -113,12 +170,14 @@ Section Shift.
 
   Definition Shift_L (s : sig) := Mirror (Shift s).
 
-  
+
   Definition Shift_L_fun_measure (t : tape sig) := length (tape_local_l t).
 
   Function Shift_L_fun (s : sig) (t : tape sig) {measure Shift_L_fun_measure t} :=
     match current t with
-    | Some c => Shift_L_fun c (doAct t (Some s, L))
+    | Some c =>
+      if f c then doAct t (Some s, N)
+      else Shift_L_fun c (doAct t (Some s, L))
     | None => tape_write t (Some s)
     end.
   Proof. intros. destruct t; cbn in *; inv teq. unfold Shift_L_fun_measure. simpl_tape. omega. Qed.
@@ -143,11 +202,17 @@ Section Shift.
       intros -> % mirror_tape_inv_midtape.
       rewrite Shift_L_fun_equation; cbn. reflexivity.
     - revert s rs m t'. induction ls as [ | l ls' IH]; intros; cbn in *.
-      + do 2 (rewrite Shift_fun_equation in H; cbn in H). apply mirror_tape_inv_midtape in H as ->.
-        now do 2 (rewrite Shift_L_fun_equation; cbn).
+      + do 2 (rewrite Shift_fun_equation in H; cbn in H).
+        destruct (f m) eqn:Em.
+        * apply mirror_tape_inv_midtape in H as ->.
+          do 1 (rewrite Shift_L_fun_equation; cbn). now rewrite Em.
+        * apply mirror_tape_inv_midtape in H as ->.
+          do 2 (rewrite Shift_L_fun_equation; cbn). now rewrite Em.
       + do 1 (rewrite Shift_fun_equation in H; cbn in H).
         do 1 (rewrite Shift_L_fun_equation; cbn).
-        specialize IH with (1 := H). auto.
+        destruct (f m) eqn:Em.
+        * now apply mirror_tape_inv_midtape in H as ->.
+        * specialize IH with (1 := H). auto.
   Qed.
 
 
@@ -161,35 +226,51 @@ Section Shift.
     }
   Qed.
 
-  
+
   Lemma Shift_L_fun_correct_midtape s l ls m rs :
+    f m = false ->
+    f l = false ->
+    (forall x, In x ls -> f x = false) ->
     Shift_L_fun s (midtape (ls ++ [l]) m rs) =
     midtape nil l (rev ls ++ m :: s :: rs).
   Proof.
     revert s rs m. induction ls as [ | l' ls IH]; intros; cbn in *.
-    - do 3 (rewrite Shift_L_fun_equation; cbn). simpl_tape. reflexivity.
-    - do 1 (rewrite Shift_L_fun_equation; cbn). rewrite <- !app_assoc. cbn. now rewrite IH.
+    - do 3 (rewrite Shift_L_fun_equation; cbn). now rewrite H, H0.
+    - do 1 (rewrite Shift_L_fun_equation; cbn). rewrite <- !app_assoc. cbn. rewrite H. rewrite IH; eauto.
   Qed.
 
+  Lemma Shift_L_fun_correct_midtape_stop s ls m rs l h ls' :
+    f m = false ->
+    f l = false ->
+    f h = true ->
+    (forall x, In x ls -> f x = false) ->
+    Shift_L_fun s (midtape (ls ++ l :: h :: ls') m rs) =
+    midtape ls' l (rev ls ++ m :: s :: rs).
+  Proof.
+    revert s rs m. induction ls as [ | l' ls IH]; intros; cbn in *.
+    - do 3 (rewrite Shift_L_fun_equation; cbn). rewrite H, H0, H1. reflexivity.
+    - do 1 (rewrite Shift_L_fun_equation; cbn). rewrite <- !app_assoc. cbn. rewrite H. rewrite IH; eauto.
+  Qed.
 
   Lemma Shift_L_TerminatesIn (s : sig) :
     projT1 (Shift_L s) ↓
-           (fun tin k => 4 + 4 * length (tape_local_l tin[@Fin0]) <= k).
+           (fun tin k => Shift_steps (tape_local_l tin[@Fin0]) <= k).
   Proof.
     eapply TerminatesIn_monotone.
     { unfold Shift_L. TM_Correct. apply Shift_TerminatesIn. }
     { intros tin k Hk. hnf. now simpl_tape in *. }
   Qed.
 
+
 End Shift.
 
 
 Ltac smpl_TM_Shift :=
   lazymatch goal with
-  | [ |- Shift   _ ⊨ _ ] => eapply Shift_Realise
-  | [ |- Shift_L _ ⊨ _ ] => eapply Shift_L_Realise
-  | [ |- projT1 (Shift   _) ↓ _ ] => eapply Shift_TerminatesIn
-  | [ |- projT1 (Shift_L _) ↓ _ ] => eapply Shift_L_TerminatesIn
+  | [ |- Shift   _ _ ⊨ _ ] => eapply Shift_Realise
+  | [ |- Shift_L _ _ ⊨ _ ] => eapply Shift_L_Realise
+  | [ |- projT1 (Shift   _ _) ↓ _ ] => eapply Shift_TerminatesIn
+  | [ |- projT1 (Shift_L _ _) ↓ _ ] => eapply Shift_L_TerminatesIn
   end.
 
 Smpl Add smpl_TM_Shift : TM_Correct.
